Added custom array translations.

eve/Src/Delivery/studio/tools/autoproof/arrays.bpl
@@ -32,10 +32,12 @@ axiom (forall h: HeapType, a: ref, i: int ::
 
 // Invariant for array objects
 function ARRAY.$inv(h: HeapType, a: ref) returns (bool) {
-	(h[a, ARRAY.lower] == 1) && 
-	(h[a, ARRAY.upper] >= 0) && 
-	(h[a, ARRAY.count] >= 0) && 
-	(h[a, ARRAY.count] == h[a, ARRAY.upper] - h[a, ARRAY.lower] + 1)
+	(a != Void) ==> (
+		(h[a, ARRAY.lower] == 1) && 
+		(h[a, ARRAY.upper] >= 0) && 
+		(h[a, ARRAY.count] >= 0) && 
+		(h[a, ARRAY.count] == h[a, ARRAY.upper] - h[a, ARRAY.lower] + 1)
+	)
 }
 
 function ARRAY#ref#.$inv(h: HeapType, a: ref, ct: Type) returns (bool) {
@@ -54,13 +56,13 @@ procedure ARRAY#int#.make(
 			l: int where is_integer_32(l),
 			u: int where is_integer_32(u)
 		);
-	requires l <= u + 1;
+	requires l <= u + 1; // pre line:1
 	ensures Heap[c, ARRAY.lower] == l;
 	ensures Heap[c, ARRAY.upper] == u;
 	ensures ARRAY.$inv(Heap, c);
 	ensures (forall i: int :: ARRAY.$is_index(Heap, c, i) ==> ARRAY.$item(Heap, c, i) == 0);
 	modifies Heap;
-	ensures (forall<beta> o: ref, f: Field beta :: (o != c) ==> (Heap[o, f] == old(Heap)[o, f]));
+	ensures (forall<beta> o: ref, f: Field beta :: (o != c || (f != ARRAY.lower && f != ARRAY.upper && f != ARRAY.count && f != $area)) ==> (Heap[o, f] == old(Heap)[o, f]));
 
 procedure ARRAY#int#.make_filled(
 			c: ref where attached(Heap, c, ARRAY#int#),
@@ -75,6 +77,71 @@ procedure ARRAY#int#.make_filled(
 	ensures (forall i: int :: ARRAY.$is_index(Heap, c, i) ==> ARRAY.$item(Heap, c, i) == v);
 	modifies Heap;
 	ensures (forall<beta> o: ref, f: Field beta :: (o != c) ==> (Heap[o, f] == old(Heap)[o, f]));
+
+procedure ARRAY#int#.put(
+			c: ref where attached(Heap, c, ARRAY#int#),
+			item: int where is_integer_32(item),
+			pos: int where is_integer_32(pos)
+		);
+	requires ARRAY.$is_index(Heap, c, pos); // pre line:1
+	ensures ARRAY.$item(Heap, c, pos) == item;
+	ensures ARRAY.$inv(Heap, c);
+	modifies Heap;
+	ensures (forall<beta> o: ref, f: Field beta :: (o != c || f != $area) ==> (Heap[o, f] == old(Heap)[o, f]));
+	ensures (forall i: int :: (ARRAY.$is_index(Heap, c, i) && i != pos) ==> ARRAY.$item(Heap, c, i) == old(ARRAY.$item(Heap, c, i)));
+
+procedure ARRAY#int#.item(
+			c: ref where attached(Heap, c, ARRAY#int#),
+			pos: int where is_integer_32(pos)
+		) returns (result: int);
+	requires ARRAY.$is_index(Heap, c, pos); // pre line:1
+	ensures result == ARRAY.$item(Heap, c, pos);
+
+procedure ARRAY#int#.count(
+			c: ref where attached(Heap, c, ARRAY#int#)
+		) returns (result: int);
+	ensures result == Heap[c, ARRAY.count];
+
+function fun.ARRAY#int#.count(heap: HeapType, c: ref) returns (int) {
+	heap[c, ARRAY.count]
+}
+
+procedure ARRAY#int#.has(
+			c: ref where attached(Heap, c, ARRAY#int#),
+			val: int where is_integer_32(val)
+		) returns (result: bool);
+	ensures result == (exists i: int :: (ARRAY.$is_index(Heap, c, i) && (ARRAY.$item(Heap, c, i) == val)));
+
+axiom (forall heap: HeapType, c: ref :: (fun.ARRAY#int#.count(heap, c) == 0) ==> (!(exists i: int :: ARRAY.$is_index(heap, c, i))));
+
+function fun.ARRAY#int#.has(heap: HeapType, c: ref, val: int) returns (bool) {
+	(exists i: int :: (ARRAY.$is_index(heap, c, i) && (ARRAY.$item(heap, c, i) == val)))
+}
+
+function fun.ARRAY#int#.has_not(heap: HeapType, c: ref, val: int) returns (bool) {
+	(forall i: int :: (ARRAY.$is_index(heap, c, i) ==> !(ARRAY.$item(heap, c, i) == val)))
+}
+
+
+procedure ARRAY#int#.subarray(
+			c: ref where attached(Heap, c, ARRAY^INTEGER_32^),
+			l: int where is_integer_32(l),
+			u: int where is_integer_32(u)
+		) returns (result: ref);
+	requires 1 <= l && l <= fun.ARRAY#int#.count(Heap, c) + 1;
+	requires 0 <= u && u <= fun.ARRAY#int#.count(Heap, c);
+//	requires (l <= u) || (l == u + 1);
+	ensures (forall o: ref :: old(Heap)[o, $allocated] ==> o != result);
+	ensures attached(Heap, result, ARRAY^INTEGER_32^);
+	ensures ARRAY.$inv(Heap, result);
+	ensures Heap[result, ARRAY.lower] == 1;
+	ensures Heap[result, ARRAY.count] == (u - l + 1);
+	ensures 0 <= fun.ARRAY#int#.count(Heap, result) && fun.ARRAY#int#.count(Heap, result) <= fun.ARRAY#int#.count(Heap, c);
+	ensures (forall i: int :: ARRAY.$is_index(Heap, result, i) ==> ARRAY.$item(Heap, result, i) == ARRAY.$item(Heap, c, i + l - 1));
+	ensures (forall i: int :: ARRAY.$is_index(Heap, result, i) ==> ARRAY.$item(Heap, result, i) == ARRAY.$item(Heap, c, i + l - 1));
+	modifies Heap;
+	ensures (forall<beta> o: ref, f: Field beta :: (o != result) ==> (Heap[o, f] == old(Heap)[o, f]));
+
 
 procedure ARRAY#ref#.make(
 			c: ref where attached(Heap, c, ARRAY#ref#),
