eve/Src/framework/eiffel2boogie/translation/custom/e2b_custom_array_call_handler.e
@@ -25,11 +25,37 @@ feature -- Basic operations
 	handle_routine_call_in_body (a_translator: E2B_BODY_EXPRESSION_TRANSLATOR; a_feature: FEATURE_I; a_parameters: BYTE_LIST [PARAMETER_B])
 			-- <Precursor>
 		do
+			if a_feature.feature_name ~ "make" then
+				a_translator.process_builtin_routine_call (a_feature, a_parameters, "ARRAY#int#.make")
+			elseif a_feature.feature_name ~ "put" then
+				a_translator.process_builtin_routine_call (a_feature, a_parameters, "ARRAY#int#.put")
+			elseif a_feature.feature_name ~ "item" then
+				a_translator.process_builtin_routine_call (a_feature, a_parameters, "ARRAY#int#.item")
+			elseif a_feature.feature_name ~ "count" then
+				a_translator.process_builtin_routine_call (a_feature, a_parameters, "ARRAY#int#.count")
+			elseif a_feature.feature_name ~ "has" then
+				a_translator.process_builtin_routine_call (a_feature, a_parameters, "ARRAY#int#.has")
+			elseif a_feature.feature_name ~ "subarray" then
+				a_translator.process_builtin_routine_call (a_feature, a_parameters, "ARRAY#int#.subarray")
+			end
 		end
 
 	handle_routine_call_in_contract (a_translator: E2B_CONTRACT_EXPRESSION_TRANSLATOR; a_feature: FEATURE_I; a_parameters: BYTE_LIST [PARAMETER_B])
 			-- <Precursor>
 		do
+			if a_feature.feature_name ~ "make" then
+				a_translator.process_builtin_routine_call (a_feature, a_parameters, "fun.ARRAY#int#.make")
+			elseif a_feature.feature_name ~ "put" then
+				a_translator.process_builtin_routine_call (a_feature, a_parameters, "fun.ARRAY#int#.put")
+			elseif a_feature.feature_name ~ "item" then
+				a_translator.process_builtin_routine_call (a_feature, a_parameters, "ARRAY.$item")
+			elseif a_feature.feature_name ~ "has" then
+				a_translator.process_builtin_routine_call (a_feature, a_parameters, "fun.ARRAY#int#.has")
+			elseif a_feature.feature_name ~ "count" then
+				a_translator.process_builtin_routine_call (a_feature, a_parameters, "fun.ARRAY#int#.count")
+			elseif a_feature.feature_name ~ "subarray" then
+				a_translator.process_builtin_routine_call (a_feature, a_parameters, "fun.ARRAY#int#.subarray")
+			end
 		end
 
 end
