eve/Src/framework/eiffel2boogie/translation/e2b_body_expression_translator.e
@@ -72,7 +72,7 @@ feature -- Visitors
 			check l_type /= Void end
 			l_feature := a_node.type.associated_class.feature_of_rout_id (a_node.call.routine_id)
 			check feature_valid: l_feature /= Void end
-			translation_pool.add_referenced_feature (l_feature, l_type)
+--			translation_pool.add_referenced_feature (l_feature, l_type)
 
 			create_local (l_type)
 
@@ -106,7 +106,7 @@ feature -- Visitors
 				process_routine_call (l_feature, a_node.parameters)
 			end
 
-			process_routine_call (l_feature, a_node.parameters)
+--			process_routine_call (l_feature, a_node.parameters)
 
 			current_target := l_target
 			current_target_type := l_target_type
@@ -223,6 +223,43 @@ feature -- Translation
 			translation_pool.add_referenced_feature (a_feature, current_target_type)
 
 			create l_call.make (name_translator.boogie_name_for_feature (a_feature, current_target_type))
+			l_call.add_argument (current_target)
+
+				-- Process arguments in context of feature
+			l_target := current_target
+			l_target_type := current_target_type
+			last_expression := Void
+
+			current_target := entity_mapping.current_entity
+			current_target_type := context_type
+
+			procedure_calls.extend (l_call)
+			safe_process (a_parameters)
+			procedure_calls.remove
+
+			current_target := l_target
+			current_target_type := l_target_type
+
+				-- Process call
+			if a_feature.has_return_value then
+				create_local (a_feature.type.instantiated_in (current_target_type))
+				l_call.set_target (last_local)
+				last_expression := last_local
+			else
+					-- No expression generated, this has to be a call statement
+				last_expression := Void
+			end
+			side_effect.extend (l_call)
+		end
+
+	process_builtin_routine_call (a_feature: FEATURE_I; a_parameters: BYTE_LIST [PARAMETER_B]; a_builtin_name: STRING)
+			-- Process feature call.
+		local
+			l_target: IV_EXPRESSION
+			l_target_type: TYPE_A
+			l_call: IV_PROCEDURE_CALL
+		do
+			create l_call.make (a_builtin_name)
 			l_call.add_argument (current_target)
 
 				-- Process arguments in context of feature
